DecoupledConsensus/Store/Proof/Properties.lean
@@ -151,10 +151,10 @@ theorem parentFirstReplay_liveComplete_property {f : ℕ} :
 theorem parentFirstReplay_getConfirmed_property {f : ℕ} :
     ParentFirstReplayGetConfirmedStatement n f := by
   intro hn hNoSlash input₁ input₂ S T B hReplayS hReplayT hPFS
-    hPFT hNoDupS hNoDupT hNoGenesisS hNoGenesisT hInputIdS hInputEq
+    hPFT hNoDupS hNoDupT hNoGenesisS hNoGenesisT hInputIdS hInputBlockEq
   exact parentFirstReplay_getConfirmed_order_independent hn hNoSlash
     hReplayS hReplayT hPFS hPFT hNoDupS hNoDupT hNoGenesisS hNoGenesisT
-    hInputIdS hInputEq
+    hInputIdS hInputBlockEq
 
 end Store
 
